pulse/src/checker/Pulse.Syntax.Base.fst
@@ -141,8 +141,8 @@ let rec eq_pattern (p1 p2 : pattern) : b:bool{ b <==> (p1 == p2) } =
   match p1, p2 with
   | Pat_Cons f1 vs1,
     Pat_Cons f2 vs2 ->
+    FStar.Sealed.sealed_singl f1.fv_range f2.fv_range;
     f1.fv_name = f2.fv_name &&
-    f1.fv_range = f2.fv_range &&
     eq_list_dec p1 p2 eq_sub_pat vs1 vs2
 
   | Pat_Constant c1, Pat_Constant c2 ->
@@ -179,7 +179,9 @@ let eq_hint_type (ht1 ht2:proof_hint_type)
       eq_tm_opt tac_opt tac_opt2 &&
       e1 = e2
     | WILD, WILD -> true
-    | SHOW_PROOF_STATE r1, SHOW_PROOF_STATE r2 -> r1 = r2
+    | SHOW_PROOF_STATE r1, SHOW_PROOF_STATE r2 ->
+      FStar.Sealed.sealed_singl r1 r2;
+      true
     | _ -> false
 
 let eq_ascription (a1 a2:comp_ascription) 
